\begin{figure}[h!]\centering
\begin{spacing}{1.6}
  \begin{tabular}{rclr}
    \eval{$\mathit{cst}$}{$\mem$} &=& $\mathit{cst}$ & \eqlabel{E-cst} \\

    \eval{$\mathit{x}$}{$(\env, \store)$} &=& $\store(\env(\mathit{x}))$
    & \eqlabel{E-lval} \\

    \eval{$\mathit{x}$\lstinline'['$h$\lstinline']'}{$(\env, \store)$}
    &=&
    $\store(\env(\mathit{x}$
    \lstinline'['\eval{$h$}{$(\env, \store)$}\lstinline']'$))$
    & \eqlabel{E-deref} \\

    \eval{$\mathit{unop}~h$}{$\mem$}
    &=& $\mathit{unop}$ (\eval{$h$}{$\mem$}) & \eqlabel{E-unop} \\

    \eval{$h_1~\mathit{binop}~h_2$}{$\mem$}
    &=& (\eval{$h_1$}{$\mem$}) $\mathit{binop}$
    (\eval{$h_2$}{$\mem$}) & \eqlabel{E-binop} \\

    \eval{\lstinline'\\abs('$t$\lstinline')'}{$\mem$} &=&
    $\lvert$ \eval{$t$}{$\mem$} $\rvert$ & \eqlabel{E-abs} \\

    \multicolumn{4}{l}{
      \eval{\lstinline'\\sum('$t_1$, $t_2$,
        \lstinline'\\lambda integer' $k \semicolon t_3$ \lstinline')'}{$\mem$}
    } \\
    &=&
    $\Sigma'(\mbox{\eval{$t_1$}{$\mem$}},\mbox{\eval{$t_2$}{$\mem$}},(\lambda~k.\mbox{\eval{$t_3$}{$\mem$}}))$
    & \eqlabel{E-sum} \\
    \multicolumn{4}{c}{
      où $\Sigma'(v_1,v_2,f) = \sum_{i = v_1}^{v_2} f(i)$
    } \\

    \multicolumn{4}{l}{
      \eval{\lstinline'\\product('$t_1$, $t_2$,
        \lstinline'\\lambda integer' $k \semicolon t_3$ \lstinline')'}{$\mem$}
    } \\
    &=&
    $\Pi'(\mbox{\eval{$t_1$}{$\mem$}},\mbox{\eval{$t_2$}{$\mem$}},(\lambda~k.\mbox{\eval{$t_3$}{$\mem$}}))$
    & \eqlabel{E-prod} \\
    \multicolumn{4}{c}{
      où $\Pi'(v_1,v_2,f) = \prod_{i = v_1}^{v_2} f(i)$
    } \\

    \multicolumn{4}{l}{
      \eval{\lstinline'\\numof('$t_1$, $t_2$,
        \lstinline'\\lambda integer' $k \semicolon t_3$ \lstinline')'}{$\mem$}
    } \\
    &=&
    $N'(\mbox{\eval{$t_1$}{$\mem$}},\mbox{\eval{$t_2$}{$\mem$}},(\lambda~k.\mbox{\eval{$t_3$}{$\mem$}}))$
    & \eqlabel{E-num} \\
    \multicolumn{4}{c}{
      où $N'(v_1,v_2,f) = \sum_{i = v_1}^{v_2} (f(i) ? 1 : 0)$
    } \\

    \eval{$h_1$ \texttt{?} $h_2$ \texttt{:} $h_3$}{$\mem$}
    &=& \eval{$h_2$}{$\mem$} si (\eval{$h_1$}{$\mem$}) $\neq 0$,
    & \eqlabel{E-tif} \\
    & & \eval{$h_3$}{$\mem$} sinon & \\

    \eval{\lstinline'\\old('$t$\lstinline')'}{$\mem$}
    &=& \eval{$t$}{$\mem_{Beg_{\mathtt{f}}}$}
    & \eqlabel{E-old} \\

    \eval{\lstinline'\\null'}{$\mem$} &=& \lstinline'NULL'
    & \eqlabel{E-null} \\

    \eval{\lstinline'\\result'}{$\mem$}
    &=& \eval{\lstinline'res'}{$\mem$} & \eqlabel{E-res} \\
  \end{tabular}
  \caption{Sémantique dénotationnelle des termes et expressions}
  \label{fig:sem-exp-term}
\end{spacing}
\end{figure}
