\begin{figure}[h!]\centering
\begin{spacing}{1.6}
  \begin{tabular}{rclr}
    \eval{\lstinline'\\true'}{$\mem$} &=& $1$ & \eqlabel{P-true} \\
    \eval{\lstinline'\\false'}{$\mem$} &=& $0$ & \eqlabel{P-false} \\
    \eval{\lstinline'\\valid('$x$\lstinline')'}{$(\env, \store)$}
    &=& $0$ si $\env(x) = \bot$,
    $1$ sinon & \eqlabel{P-valid} \\
    \eval{\lstinline'\\valid('$x$\lstinline'+('$\mathit{t_1}$
      \lstinline'..'$\mathit{t_2}$\lstinline'))'}{$\mem$} &=&
    \eval{
      \lstinline'\\valid('$x$\lstinline'+'$\mathit{t_1}$\lstinline')'
      \lstinline'\&\&' $\ldots$ \lstinline'\&\&'
      \lstinline'\\valid('$x$\lstinline'+'$\mathit{t_2}$\lstinline')'
    }{$\mem$}
    & \eqlabel{P-validr} \\

    \multicolumn{4}{l}{
      \eval{\lstinline'\\forall integer' $k \semicolon t_1$ \lstinline'<=' $k$
        \lstinline'<=' $t_2$ \lstinline'==>' $p$}{$\mem$}
    }\\
    &=&
    $F'(\mbox{\eval{$t_1$}{$\mem$}}, \mbox{\eval{$t_2$}{$\mem$}},(\lambda~k.\mbox{\eval{$p$}{$\mem$}}))$
    & \eqlabel{P-forall} \\
    \multicolumn{4}{c}{
      où $F'(v_1,v_2,f) = \forall i. (v_1 \le i \le v_2 \Rightarrow f(i))$
    } \\

    \multicolumn{4}{l}{
      \eval{\lstinline'\\exists integer' $k \semicolon t_1$ \lstinline'<=' $k$
        \lstinline'<=' $t_2$ \lstinline'\&\&' $p$}{$\mem$}
    }\\
    &=&
    $E'(\mbox{\eval{$t_1$}{$\mem$}}, \mbox{\eval{$t_2$}{$\mem$}},(\lambda~k.\mbox{\eval{$p$}{$\mem$}}))$
    & \eqlabel{P-exists} \\
    \multicolumn{4}{c}{
      où $E'(v_1,v_2,f) = \exists i. (v_1 \le i \le v_2 \land f(i))$
    } \\

    \eval{\lstinline'\!'$p$}{$\mem$} &=& $\lnot$ (\eval{$p$}{$\mem$})
    & \eqlabel{P-not} \\
    \eval{$p_1$ \lstinline'\&\&' $p_2$}{$\mem$} &=&
    (\eval{$p_1$}{$\mem$}) $\land$ (\eval{$p_2$}{$\mem$})
    & \eqlabel{P-and} \\
    \eval{$p_1$ \lstinline'||' $p_2$}{$\mem$} &=&
    (\eval{$p_1$}{$\mem$}) $\lor$ (\eval{$p_2$}{$\mem$})
    & \eqlabel{P-or} \\
    \eval{$p_1$ \lstinline'==>' $p_2$}{$\mem$} &=&
    (\eval{$p_1$}{$\mem$}) $\Rightarrow$ (\eval{$p_2$}{$\mem$})
    & \eqlabel{P-impl} \\
    \eval{$p_1$ \lstinline'<==>' $p_2$}{$\mem$} &=&
    (\eval{$p_1$}{$\mem$}) $\Leftrightarrow$(\eval{$p_2$}{$\mem$})
    & \eqlabel{P-eq} \\
    \eval{$t$ \texttt{?} $p_1$ \texttt{:} $p_2$}{$\mem$} &=&
    \eval{$p_1$}{$\mem$} si (\eval{$t$}{$\mem$}) $\neq 0$,
    \eval{$p_2$}{$\mem$} sinon
    & \eqlabel{P-pif} \\
    \eval{$t_1~\mathit{rel}~t_2$}{$\mem$}
    &=& (\eval{$t_1$}{$\mem$}) $\mathit{rel}$
    (\eval{$t_2$}{$\mem$}) & \eqlabel{P-rel} \\
  \end{tabular}
  \caption{Sémantique dénotationnelle des prédicats}
  \label{fig:sem-pred}
\end{spacing}
\end{figure}
